clean-ups around normalisation

theories/Decidability.v
@@ -4,7 +4,7 @@ From LogRel Require Import Utils Syntax.All DeclarativeTyping GenericTyping
   AlgorithmicTyping BundledAlgorithmicTyping AlgorithmicConvProperties
   AlgorithmicTypingProperties PropertiesDefinition NeutralConvProperties LogRelConsequences.
 
-From LogRel.Decidability Require Import Functions Soundness Completeness Termination.
+From LogRel.Decidability Require Import Functions Soundness NegativeSoundness Termination.
 From PartialFun Require Import Monad PartialFun MonadExn.
 
 Import AlgorithmicTypingProperties DeclarativeTypingProperties.
@@ -12,12 +12,10 @@ Set Universe Polymorphism.
 
 Import IntermediateTypingProperties BundledTypingData.
 
-#[local]Existing Instance TypingSubstLogRel.
-#[local]Existing Instance RedCompleteLogRel.
-#[local]Existing Instance TypeConstructorsInjLogRel.
-#[local]Existing Instance NormalisationLogRel.
-#[local]Existing Instance ConvCompleteLogRel.
-#[local]Existing Instance TypingCompleteLogRel.
+#[local]Existing Instances
+  TypingSubstLogRel RedCompleteLogRel TypeConstructorsInjLogRel
+  TermConstructorsInjLogRel ConvNeutralConvPosLogRel
+  NormalisationLogRel ConvCompleteLogRel CompleteAlgoNormalisation.
 
 Definition inspect {A} (a : A) : ∑ b, a = b :=
   (a;eq_refl).
@@ -28,7 +26,7 @@ Notation "x 'eqn:' p" := ((x;p)) (only parsing, at level 20).
 Obligation Tactic := idtac.
 
 Equations check (Γ : context) (t T : term) (hΓ : [|- Γ]) (hT : [Γ |- T]) :
-  [Γ |- t : T] + ~[Γ |- t : T] :=
+  [Γ |-[de] t : T] + ~[Γ |-[de] t : T] :=
 
 check Γ t T hΓ hT with (inspect (def (typing tconv) (check_state;Γ;T;t) _)) :=
   {
@@ -38,7 +36,7 @@ check Γ t T hΓ hT with (inspect (def (typing tconv) (check_state;Γ;T;t) _)) :
 Next Obligation.
   intros.
   apply typing_terminates ; tea.
-  - apply implem_tconv_sound.
+  - intros. now apply implem_tconv_sound.
   - now intros ; eapply tconv_terminates.
 Qed.
 Next Obligation.
@@ -55,20 +53,10 @@ Next Obligation.
   set (Hter := check_obligations_obligation_1 _ _ _ _ _) in *.
   clearbody Hter.
   pose proof (def_graph_sound _ _ Hter) as Hgraph.
-  enough (graph (typing tconv) (check_state;Γ;T;t) ok).
-  {
-    eapply orec_graph_functional in Hgraph ; tea.
-    assert (ok = exception e0) as [=] by (etransitivity ; eassumption).
-  }
-
-  change [Γ |-[de] t : T] in Hty.
-  eapply (tm_compl (ta' := bn)) in Hty as [].
-
-  apply typing_complete.
-  1: now apply implem_conv_complete.
-  constructor ; tea.
-  econstructor ; tea.
-  now apply ty_conv_compl.
+  rewrite e in Hgraph.
+  eapply implem_typing_sound_neg in Hgraph ; cbn in * ; eauto.
+  + eapply implem_tconv_sound.
+  + intros ; eapply implem_tconv_sound_neg ; tea.
 Qed.
 
 Print Assumptions check.
