theories/TypingProperties/Normalisation.v
@@ -1,0 +1,207 @@
+(** * LogRel.Normalisation: definition and properties of normalisation. *)
+From Coq Require Import CRelationClasses ssrbool.
+From LogRel Require Import Utils Syntax.All GenericTyping DeclarativeTyping.
+
+Record normalising (t : term) := {
+  norm_val : term;
+  norm_red : [ t ⤳* norm_val ];
+  norm_whnf : whnf norm_val;
+}.
+
+(** Deep normalisation, based on a type to incorporate η laws *)
+
+(** Deeply normalising terms (at a given type) *)
+Inductive dnorm_tm : context -> term -> term -> Type :=
+| termDeepRed {Γ t t' A A'} :
+  [A ⤳* A'] ->
+  [t ⤳* t'] ->
+  dnf_tm Γ A' t' ->
+  dnorm_tm Γ A t
+(** Deep normal forms (whnf, recursively containing normalising subterms) *)
+with dnf_tm : context -> term -> term -> Type :=
+| termDeepPi {Γ A B} :
+    dnorm_tm Γ U A ->
+    dnorm_tm (Γ,,A) U B ->
+    dnf_tm Γ U (tProd A B)
+| termDeepNat {Γ} :
+    dnf_tm Γ U tNat
+| termDeepZero {Γ} :
+    dnf_tm Γ tNat tZero
+| termDeepSucc {Γ t} :
+    dnorm_tm Γ tNat t ->
+    dnf_tm Γ tNat (tSucc t)
+| termDeepEmpty {Γ} :
+    dnf_tm Γ U tEmpty
+| termDeepFun {Γ f A B} :
+    whnf f ->
+    dnorm_tm (Γ,,A) B (eta_expand f) ->
+    dnf_tm Γ (tProd A B) f
+| termDeepSig {Γ A B} :
+    dnorm_tm Γ U A ->
+    dnorm_tm (Γ,,A) U B ->
+    dnf_tm Γ U (tSig A B)
+| termDeepPair {Γ p A B} :
+  whnf p ->
+  dnorm_tm Γ A (tFst p) ->
+  dnorm_tm Γ B[(tFst p)..] (tSnd p) ->
+  dnf_tm Γ (tSig A B) p
+| termDeepId {Γ A x y} :
+  dnorm_tm Γ U A ->
+  dnorm_tm Γ A x ->
+  dnorm_tm Γ A y ->
+  dnf_tm Γ U (tId A x y)
+| termDeepRefl {Γ A A' x x' y} :
+  dnf_tm Γ (tId A' x' y) (tRefl A x)
+| termDeepNeu {Γ m T P} :
+  isPosType P ->
+  dneu Γ T m ->
+  dnf_tm Γ P m
+(** Deep neutrals (wh neutrals, with recursively normalising/neutral subterms).
+    Note that the type is "inferred". *)    
+with dneu : context -> term -> term -> Type :=
+| neuDeepVar {Γ n decl} :
+  in_ctx Γ n decl ->
+  dneu Γ decl (tRel n)
+| neuDeepApp {Γ n t A B} :
+  dneu_red Γ (tProd A B) n ->
+  dnorm_tm Γ A t ->
+  dneu Γ B[t..] (tApp n t)
+| neuDeepNatElim {Γ n P hz hs} :
+  dneu_red Γ tNat n ->
+  dnorm_ty (Γ,,tNat) P ->
+  dnorm_tm Γ P[tZero..] hz ->
+  dnorm_tm Γ (elimSuccHypTy P) hs ->
+  dneu Γ P[n..] (tNatElim P hz hs n)
+| neuDeepEmptyElim {Γ P n} :
+  dneu_red Γ tEmpty n ->
+  dnorm_ty (Γ,,tEmpty) P ->
+  dneu Γ P[n..] (tEmptyElim P n)
+| neuDeepFst {Γ n A B} :
+  dneu_red Γ (tSig A B) n ->
+  dneu Γ A (tFst n)
+| neuDeepSnd {Γ n A B} :
+  dneu_red Γ (tSig A B) n ->
+  dneu Γ B[(tFst n)..] (tSnd n)
+| neuDeepIdElim {Γ A A' x x' P hr y y' n} :
+  dneu_red Γ (tId A' x' y') n ->
+  dnorm_ty (Γ ,, A ,, tId A⟨@wk1 Γ A⟩ x⟨@wk1 Γ A⟩ (tRel 0)) P ->
+  dnorm_tm Γ P[tRefl A x .: x..] hr ->
+  dneu Γ P[n .: y..] (tIdElim A x P hr y n)
+
+with dneu_red : context -> term -> term -> Type :=
+| neuDeepRed {Γ n A A'} :
+  dneu Γ A n ->
+  [A ⤳* A'] ->
+  whnf A' ->
+  dneu_red Γ A' n
+
+(** Deeply normalising types *)
+with dnorm_ty : context -> term -> Type :=
+| typeDeepNorm {Γ A A'} :
+  [A ⤳* A'] ->
+  dnf_ty Γ A' ->
+  dnorm_ty Γ A
+(** **** Conversion of types reduced to weak-head normal forms *)
+with dnf_ty : context -> term -> Type :=
+| typeDeepU {Γ} :
+  dnf_ty Γ U
+| typeDeepPi {Γ A B} :
+  dnorm_ty Γ A ->
+  dnorm_ty (Γ,,A) B ->
+  dnf_ty Γ (tProd A B)
+| typeDeepNat {Γ} :
+  dnf_ty Γ tNat
+| typeDeepEmpty {Γ} :
+  dnf_ty Γ tEmpty
+| typeDeepSig {Γ A B} :
+  dnorm_ty Γ A ->
+  dnorm_ty (Γ,,A) B ->
+  dnf_ty Γ (tSig A B)
+| typeDeepId {Γ A x y} :
+  dnorm_ty Γ A ->
+  dnorm_tm Γ A x ->
+  dnorm_tm Γ A y ->
+  dnf_ty Γ (tId A x y)
+| typeDeepNeu {Γ m T} :
+  dneu Γ T m ->
+  dnf_ty Γ m.
+
+Section InductionScheme.
+
+  Scheme 
+    Minimality for dnorm_tm Sort Type with
+    Minimality for dnf_tm   Sort Type with
+    Minimality for dneu     Sort Type with
+    Minimality for dneu_red Sort Type with
+    Minimality for dnorm_ty Sort Type with
+    Minimality for dnf_ty   Sort Type.
+
+  Combined Scheme _DeepNormInduction from
+      dnorm_tm_rect_nodep,
+      dnf_tm_rect_nodep,
+      dneu_rect_nodep,
+      dneu_red_rect_nodep,
+      dnorm_ty_rect_nodep,
+      dnf_ty_rect_nodep.
+
+  Let _DeepNormInductionType :=
+    ltac:(let ind := fresh "ind" in
+        pose (ind := _DeepNormInduction);
+        refold ;
+        let ind_ty := type of ind in
+        exact ind_ty).
+
+  Let DeepNormInductionType :=
+    ltac: (let ind := eval cbv delta [_DeepNormInductionType] zeta
+      in _DeepNormInductionType in
+      let ind' := polymorphise ind in
+    exact ind').
+
+  Lemma DeepNormInduction : DeepNormInductionType.
+  Proof.
+    intros PNormTm PNfTm PNeu PNeuRed PNormTy PNfTy **.
+    pose proof (_DeepNormInduction PNormTm PNfTm PNeu PNeuRed PNormTy PNfTy) as H.
+    destruct H as (?&?&?&?&?&?).
+    all: try (assumption ; fail).
+    repeat (split;[assumption|]); assumption.
+  Qed.
+
+  Definition DeepNormInductionConcl :=
+    ltac:(
+      let t := eval cbv delta [DeepNormInductionType] beta in DeepNormInductionType in
+      let t' := remove_steps t in
+      exact t').
+
+End InductionScheme.
+
+Lemma dnf_whnf :
+  DeepNormInductionConcl
+  (fun (Γ : context) (A t : term) => True)
+  (fun (Γ : context) (A t : term) => isType A × whnf t)
+  (fun (Γ : context) (A t : term) => whne t)
+  (fun (Γ : context) (A t : term) => whnf A × whne t)
+  (fun (Γ : context) (A : term) => True)
+  (fun (Γ : context) (A : term) => isType A).
+Proof.
+  apply DeepNormInduction.
+  all: intros ; prod_splitter ; prod_hyp_splitter ;
+    try solve [eauto using isPosType_isType | econstructor ; eauto].
+Qed.
+
+Lemma dnf_det :
+  DeepNormInductionConcl
+    (fun (Γ : context) (A t : term) => True)
+    (fun (Γ : context) (A t : term) => True)
+    (fun (Γ : context) (A t : term) => forall T, dneu Γ T t -> T = A)
+    (fun (Γ : context) (A t : term) => forall T, dneu_red Γ T t -> T = A)
+    (fun (Γ : context) (A : term) => True)
+    (fun (Γ : context) (A : term) => True).
+Proof.
+  apply DeepNormInduction.
+  all: try easy.
+  all: intros until T ; intros HT.
+  all: inversion HT ; subst ; eauto using in_ctx_inj.
+  all: match goal with | H : forall _ : _, _ -> _ = _, H' : _ |- _ => apply H in H' end.
+  1-3: congruence.
+  subst ; now eapply whred_det.
+Qed.
